$$\int_{}^{}{x\operatorname{}x\text{dx}}$$

$$u = \operatorname{}x$$

$$dv = xdx$$

$$u = \operatorname{}xdu = \left( \operatorname{}x \right)^{'}dx = 2\ln x\left( \ln x \right)^{'}dx = \frac{2\ln x}{x}\text{dx}$$

$$dv = xdxv = \int_{}^{}\text{xdx} = \frac{x^{2}}{2}$$

$$\int_{}^{}{x^{n}\text{dx}} = \frac{x^{n + 1}}{n + 1} + C$$

$$\int_{}^{}{x\operatorname{}x\text{dx}} = \frac{x^{2}\operatorname{}x}{2} - \int_{}^{}{\frac{x^{2}}{2} \cdot \frac{2\ln x}{x}\text{dx}} = \frac{x^{2}\operatorname{}x}{2} - \int_{}^{}{x\ln x\text{dx}}$$

$$u = \ln x \rightarrow du = \frac{1}{x}\text{dx}$$

$$dv = xdx \rightarrow v = \frac{x^{2}}{2}$$

$$\frac{x^{2}\operatorname{}x}{2} - \int_{}^{}{x\ln x\text{dx}} = \frac{x^{2}\operatorname{}x}{2} - \left( \frac{x^{2}\ln x}{2} - \int_{}^{}{\frac{x^{2}}{2} \cdot \frac{1}{x}\text{dx}} \right) = \frac{x^{2}\operatorname{}x}{2} - \frac{x^{2}\ln x}{2} + \frac{1}{2}\int_{}^{}\text{xdx} =$$

$$= \frac{x^{2}\operatorname{}x}{2} - \frac{x^{2}\ln x}{2} + \frac{1}{2} \cdot \frac{x^{2}}{2} + C = \frac{x^{2}}{2}\left( \operatorname{}x - \ln x + \frac{1}{2} \right) + C$$

$$\int_{}^{}{\frac{\ln x}{x}\text{dx}}$$

$$\int_{}^{}{\frac{\ln x}{x^{2}}\text{dx}}$$

$$\int_{}^{}{\left( x - 2 \right)e^{2x}\text{dx}}$$

$$u = x - 2 \rightarrow du = \left( x - 2 \right)^{'}dx = x$$

$$dv = e^{2x}dx \rightarrow v = \int_{}^{}{e^{2x}\text{dx}} = \frac{1}{2}e^{2x}$$

$$\int_{}^{}{\left( x - 2 \right)e^{2x}\text{dx}} = \frac{\left( x - 2 \right)e^{2x}}{2} - \frac{1}{2}\int_{}^{}{e^{2x}\text{dx}} = \frac{\left( x - 2 \right)e^{2x}}{2} - \frac{1}{2} \cdot \frac{1}{2}e^{2x} + C = \frac{e^{2x}}{2}\left( x - 2 - \frac{1}{2} \right) = \frac{e^{2x}}{2}\left( x - 1\frac{1}{2} \right)$$

$$\int_{}^{}{\left( x^{2} + x \right)e^{- x}\text{dx}}$$

$$\int_{}^{}{x\cos{6x}\text{dx}}$$

$$u = x \rightarrow du = dx$$

$$dv = \cos{6x}dx \rightarrow v = \int_{}^{}{\cos{6x}\text{dx}} = \frac{1}{6}\sin{6x}$$

$$\int_{}^{}{x\cos{6x}\text{dx}} = \frac{1}{6}x\sin{6x} - \frac{1}{6}\int_{}^{}{\sin{6x}\text{dx}} = \frac{1}{6}x\sin{6x} - \frac{1}{6} \cdot \left( - \frac{1}{6}x\cos{6x} \right) + C =$$

$$= \frac{1}{6}x\sin{6x} + \frac{1}{36}x\cos{6x} + C$$

$$\int_{}^{}{(x - 6)\sin\frac{x}{2}\text{dx}}$$

$$\int_{}^{}{\frac{x}{\operatorname{}x}\text{dx}}$$

$$u = x \rightarrow du = dx$$

$$dv = \frac{1}{\operatorname{}x}dx \rightarrow v = \int_{}^{}{\frac{1}{\operatorname{}x}\text{dx}} = - ctgx$$

$$\int_{}^{}{\frac{x}{\operatorname{}x}\text{dx}} = - xctgx + \int_{}^{}{\text{ctgx}\text{dx}} = - xctgx + \int_{}^{}{\frac{\cos x}{\sin x}\text{dx}} = - xctgx + \int_{}^{}\frac{d(\sin{x)}}{\sin x} =$$

$$= - xctgx + \ln\left| \sin x \right| + C$$

$$\int_{}^{}{x\sin x\cos x\text{dx}}$$

$$\int_{}^{}{\operatorname{atan}{2x}\text{dx}}$$

$$u = \operatorname{atan}{2x} \rightarrow du = \left( \operatorname{atan}{2x} \right)^{'}dx = \frac{1}{1 + \left( 2x \right)^{2}} \cdot \left( 2x \right)^{'}dx = \frac{2}{1 + 4x^{2}}\text{dx}$$

$$dv = dx \rightarrow v = x$$

$$\int_{}^{}{\operatorname{atan}{2x}\text{dx}} = x\operatorname{atan}{2x} - \int_{}^{}{\frac{2x}{1 + 4x^{2}}\text{dx}} = x\operatorname{atan}{2x} - \frac{1}{4}\int_{}^{}\frac{d\left( 1 + 4x^{2} \right)}{1 + 4x^{2}} =$$

$$x\operatorname{atan}{2x} - \frac{1}{4}\ln\left( 1 + 4x^{2} \right) + C$$

$$\int_{}^{}{\operatorname{asin}{3x}\text{dx}}$$

$$\int_{}^{}{x\operatorname{atan}x\text{dx}}$$
