\documentclass[]{article}
\usepackage{lmodern}
\usepackage{amssymb,amsmath}
\usepackage{ifxetex,ifluatex}
\usepackage{fixltx2e} % provides \textsubscript
\ifnum 0\ifxetex 1\fi\ifluatex 1\fi=0 % if pdftex
  \usepackage[T1]{fontenc}
  \usepackage[utf8]{inputenc}
\else % if luatex or xelatex
  \ifxetex
    \usepackage{mathspec}
  \else
    \usepackage{fontspec}
  \fi
  \defaultfontfeatures{Ligatures=TeX,Scale=MatchLowercase}
\fi
% use upquote if available, for straight quotes in verbatim environments
\IfFileExists{upquote.sty}{\usepackage{upquote}}{}
% use microtype if available
\IfFileExists{microtype.sty}{%
\usepackage[]{microtype}
\UseMicrotypeSet[protrusion]{basicmath} % disable protrusion for tt fonts
}{}
\PassOptionsToPackage{hyphens}{url} % url is loaded by hyperref
\usepackage[unicode=true]{hyperref}
\hypersetup{
            pdfborder={0 0 0},
            breaklinks=true}
\urlstyle{same}  % don't use monospace font for urls
\IfFileExists{parskip.sty}{%
\usepackage{parskip}
}{% else
\setlength{\parindent}{0pt}
\setlength{\parskip}{6pt plus 2pt minus 1pt}
}
\setlength{\emergencystretch}{3em}  % prevent overfull lines
\providecommand{\tightlist}{%
  \setlength{\itemsep}{0pt}\setlength{\parskip}{0pt}}
\setcounter{secnumdepth}{0}
% Redefines (sub)paragraphs to behave more like sections
\ifx\paragraph\undefined\else
\let\oldparagraph\paragraph
\renewcommand{\paragraph}[1]{\oldparagraph{#1}\mbox{}}
\fi
\ifx\subparagraph\undefined\else
\let\oldsubparagraph\subparagraph
\renewcommand{\subparagraph}[1]{\oldsubparagraph{#1}\mbox{}}
\fi

% set default figure placement to htbp
\makeatletter
\def\fps@figure{htbp}
\makeatother


\date{}

\begin{document}

\[\int_{}^{}{x\operatorname{}x\text{dx}}\]

\[u = \operatorname{}x\]

\[dv = xdx\]

\[u = \operatorname{}xdu = \left( \operatorname{}x \right)^{'}dx = 2\ln x\left( \ln x \right)^{'}dx = \frac{2\ln x}{x}\text{dx}\]

\[dv = xdxv = \int_{}^{}\text{xdx} = \frac{x^{2}}{2}\]

\[\int_{}^{}{x^{n}\text{dx}} = \frac{x^{n + 1}}{n + 1} + C\]

\[\int_{}^{}{x\operatorname{}x\text{dx}} = \frac{x^{2}\operatorname{}x}{2} - \int_{}^{}{\frac{x^{2}}{2} \cdot \frac{2\ln x}{x}\text{dx}} = \frac{x^{2}\operatorname{}x}{2} - \int_{}^{}{x\ln x\text{dx}}\]

\[u = \ln x \rightarrow du = \frac{1}{x}\text{dx}\]

\[dv = xdx \rightarrow v = \frac{x^{2}}{2}\]

\[\frac{x^{2}\operatorname{}x}{2} - \int_{}^{}{x\ln x\text{dx}} = \frac{x^{2}\operatorname{}x}{2} - \left( \frac{x^{2}\ln x}{2} - \int_{}^{}{\frac{x^{2}}{2} \cdot \frac{1}{x}\text{dx}} \right) = \frac{x^{2}\operatorname{}x}{2} - \frac{x^{2}\ln x}{2} + \frac{1}{2}\int_{}^{}\text{xdx} =\]

\[= \frac{x^{2}\operatorname{}x}{2} - \frac{x^{2}\ln x}{2} + \frac{1}{2} \cdot \frac{x^{2}}{2} + C = \frac{x^{2}}{2}\left( \operatorname{}x - \ln x + \frac{1}{2} \right) + C\]

\[\int_{}^{}{\frac{\ln x}{x}\text{dx}}\]

\[\int_{}^{}{\frac{\ln x}{x^{2}}\text{dx}}\]

\[\int_{}^{}{\left( x - 2 \right)e^{2x}\text{dx}}\]

\[u = x - 2 \rightarrow du = \left( x - 2 \right)^{'}dx = x\]

\[dv = e^{2x}dx \rightarrow v = \int_{}^{}{e^{2x}\text{dx}} = \frac{1}{2}e^{2x}\]

\[\int_{}^{}{\left( x - 2 \right)e^{2x}\text{dx}} = \frac{\left( x - 2 \right)e^{2x}}{2} - \frac{1}{2}\int_{}^{}{e^{2x}\text{dx}} = \frac{\left( x - 2 \right)e^{2x}}{2} - \frac{1}{2} \cdot \frac{1}{2}e^{2x} + C = \frac{e^{2x}}{2}\left( x - 2 - \frac{1}{2} \right) = \frac{e^{2x}}{2}\left( x - 1\frac{1}{2} \right)\]

\[\int_{}^{}{\left( x^{2} + x \right)e^{- x}\text{dx}}\]

\[\int_{}^{}{x\cos{6x}\text{dx}}\]

\[u = x \rightarrow du = dx\]

\[dv = \cos{6x}dx \rightarrow v = \int_{}^{}{\cos{6x}\text{dx}} = \frac{1}{6}\sin{6x}\]

\[\int_{}^{}{x\cos{6x}\text{dx}} = \frac{1}{6}x\sin{6x} - \frac{1}{6}\int_{}^{}{\sin{6x}\text{dx}} = \frac{1}{6}x\sin{6x} - \frac{1}{6} \cdot \left( - \frac{1}{6}x\cos{6x} \right) + C =\]

\[= \frac{1}{6}x\sin{6x} + \frac{1}{36}x\cos{6x} + C\]

\[\int_{}^{}{(x - 6)\sin\frac{x}{2}\text{dx}}\]

\[\int_{}^{}{\frac{x}{\operatorname{}x}\text{dx}}\]

\[u = x \rightarrow du = dx\]

\[dv = \frac{1}{\operatorname{}x}dx \rightarrow v = \int_{}^{}{\frac{1}{\operatorname{}x}\text{dx}} = - ctgx\]

\[\int_{}^{}{\frac{x}{\operatorname{}x}\text{dx}} = - xctgx + \int_{}^{}{\text{ctgx}\text{dx}} = - xctgx + \int_{}^{}{\frac{\cos x}{\sin x}\text{dx}} = - xctgx + \int_{}^{}\frac{d(\sin{x)}}{\sin x} =\]

\[= - xctgx + \ln\left| \sin x \right| + C\]

\[\int_{}^{}{x\sin x\cos x\text{dx}}\]

\[\int_{}^{}{\operatorname{atan}{2x}\text{dx}}\]

\[u = \operatorname{atan}{2x} \rightarrow du = \left( \operatorname{atan}{2x} \right)^{'}dx = \frac{1}{1 + \left( 2x \right)^{2}} \cdot \left( 2x \right)^{'}dx = \frac{2}{1 + 4x^{2}}\text{dx}\]

\[dv = dx \rightarrow v = x\]

\[\int_{}^{}{\operatorname{atan}{2x}\text{dx}} = x\operatorname{atan}{2x} - \int_{}^{}{\frac{2x}{1 + 4x^{2}}\text{dx}} = x\operatorname{atan}{2x} - \frac{1}{4}\int_{}^{}\frac{d\left( 1 + 4x^{2} \right)}{1 + 4x^{2}} =\]

\[x\operatorname{atan}{2x} - \frac{1}{4}\ln\left( 1 + 4x^{2} \right) + C\]

\[\int_{}^{}{\operatorname{asin}{3x}\text{dx}}\]

\[\int_{}^{}{x\operatorname{atan}x\text{dx}}\]

\end{document}
