СЛОЖНЫЙ ПРИМЕР

$$2 \bullet \left( \frac{3}{4} - \frac{5}{6} \right) \bullet \frac{7}{8} = 2 \bullet \left( \frac{3 \bullet 6}{4 \bullet 6} - \frac{5 \bullet 4}{6 \bullet 4} \right) \bullet \frac{7}{8} = 2 \bullet \left( \frac{18}{24} - \frac{20}{24} \right) \bullet \frac{7}{8} = 2 \bullet \left( \frac{18 - 20}{24} \right) \bullet \frac{7}{8} = 2 \bullet \left( \frac{- 2}{24} \right) \bullet \frac{7}{8} = = 2 \bullet \frac{\left( - 1 \right) \bullet 2}{24} \bullet \frac{7}{8} = \left( - 1 \right) \bullet 2 \bullet \frac{2}{24} \bullet \frac{7}{8} = \left( - 1 \right) \bullet 2 \bullet \frac{1}{12} \bullet \frac{7}{8} = \left( - 1 \right) \bullet 2 \bullet \frac{1 \bullet 7}{12 \bullet 8} = = \left( - 1 \right) \bullet 2 \bullet \frac{7}{96} = \left( - 1 \right) \bullet \frac{7 \bullet 2}{48 \bullet 2} = \left( - 1 \right) \bullet \frac{7}{48} = - \frac{7}{48}$$

Можно было поступить быстрее

$$2 \bullet \left( \frac{3 \bullet 6}{4 \bullet 6} - \frac{5 \bullet 4}{6 \bullet 4} \right) \bullet \frac{7}{8} = \left( \frac{18 - 20}{24} \right) \bullet \frac{2 \bullet 7}{8} = \frac{- 2}{24} \bullet \frac{7}{4} = - \frac{1 \bullet 7}{12 \bullet 4} = - \frac{7}{48}$$

$$8 \bullet \left( \frac{7}{6} - \frac{5}{4} \right) \bullet \frac{3}{2} = 8 \bullet \left( \frac{7 \bullet 4}{6 \bullet 4} - \frac{5 \bullet 6}{4 \bullet 6} \right) \bullet \frac{3}{2} = \left( \frac{28}{24} - \frac{30}{24} \right) \bullet \frac{8 \bullet 3}{2} = \left( \frac{28 - 30}{24} \right) \bullet \frac{24}{2} = \frac{- 2}{24} \bullet \frac{24}{2} = \frac{- 1 \bullet 2 \bullet 24}{24 \bullet 2} = - 1$$

Все задания ниже можно вычислить быстро.

Осталось понять как…

$$3.17 + 10.2 + 0.83 + 9.8 =$$

$$15.21 - 3.9 - 4.7 + 6.79 =$$

$$50 \bullet 1.34 \bullet 0.2 =$$

$$- 75.7 \bullet 0.5 \bullet 20 =$$

$$25 \bullet ( - 15.8) \bullet 4 =$$

$$0.47 \bullet 0.4 \bullet 25 =$$

$$\left( 1.25 \bullet 1.7 \bullet 0.8 - 1.7 \right) \bullet 3.45 =$$

$$3.947:\left( 3.6 - 2.6 \bullet 4 \bullet 0.25 \right) =$$

Еще задания
$$0.6\ *\ 2\ *\ ( - 3 + 5.2) - 4 =$$

$$\frac{2.7}{- 0.03} - \frac{12}{40} + 6 - ( - 3) =$$

$$\frac{128}{- 2} + 8\ *\ \left( - 8 \right) + \frac{6.8}{4} =$$

$$- 4 + \frac{20}{- 16} + \frac{4.2}{\left( - 0.7 \right)} + ( - 2) =$$

$$120 - 90\ *\ \left( - 0.02 \right) - \frac{15}{3} + \frac{96}{\left( - 4 \right)} =$$
