$5\cdot(-15)≠5\cdot(-5\cdot(-3))$

$5\cdot(-15)=5\cdot(-5\cdot3)$


$x^5\cdot(x^2)^3=$

$(x^3)^4\cdot x^8=$

$(x^4)^2\cdot(x^5)^3=$

$(x^2)^3\cdot(x^3)^5=$

$(x^3)^2\cdot(x^4)^5=$

$(x^7)^3\cdot(x^3)^4=$


$\dfrac{(2^5·(2^3)^4)}{2^{13}}=$

$\dfrac{(5^8)^2\cdot5^7}{5^{22}}=$

$\dfrac{(2^5)^2}{2^6\cdot4}=$

$\dfrac{3^7\cdot27}{(3^4)^3}=$

$\dfrac{(5^2)^4\cdot25}{5^9}=$

$\dfrac{(7^3)^3\cdot7^2}{(7^5)^2}=$

$\dfrac{3^{11}\cdot27}{(3^4)^3\cdot9}=$

$\dfrac{(11^2)^3}{11^2\cdot11^3}=$

$8x^2 x=$

$1.2abc\cdot5a=$

$3xy(-1.7)y=$

$6c^2 (-0.8)c=$

$\dfrac23 m^2 n\cdot4.5n^3=$

$2 \dfrac13 a^2 x\left(-\dfrac37\right) a^3 x^2=$

$9yy^2 y=$

$0.15pq\cdot4pq^2=$

$-8ab(-2.5) b^2=$

$10a^2 b^2 (-1.2a^3)=$

$2m^3 n\cdot0.4mn=$

$-2x^3\cdot0.5xy^2=$


$3.5\cdot3m=$

$-6ax^3\cdot9bx^2=$

$-8a^2 b^2\cdot(-8a^3 b^5)=$

$ab\cdot(-7ab^2)\cdot4a^2 b=$

$10x^2 y\cdot(-xy^2)\cdot0.6x^3=$

$-9ab^2\cdot3a^3\cdot(-4b)=$


$\dfrac27 x(1.4x^2-3.5y)=$

$-\dfrac13 c^2 (1.2d^2-6c)=$

$\dfrac12 ab(\dfrac23 a^2-\dfrac34 ab+\dfrac45 b^2)=$

$-\dfrac25 a^2 y^5 (5ay^2-\dfrac12 a^2 y-\dfrac56 a^3)=$



$-x^2 y(x^2 y^2-x^2-y^2)=$

$2.5a^2 b(4a^2-2ab+0.2b^2)=$

$(6.3x^3 y-3y^2-0.7x)\cdot10x^2 y^2=$

$-1.4p^2 q^6 (5p^3 q-1.5pq^2-2q^3)=$

$3ab(a^2-2ab+b^2)=$

$(-2ax^2+3ax-a^2)(-a^2 x^2)=$

Сравните значения выражений
 expr|sign|expr
 -|-|-
$(0.3)^{16}$ | $>$ | $(-0.3)^{16}$
$(-1.9)^{21}$ | | $(1.9)^{21}$
$-(5.6)^4$ | | $(-5.6)^4$
$(-1.4)^6$ | | $-(1.4)^6$
$-64$ | | $-2^6$
$-(0.8)^{11}$ | | $(-0.8)^{11}$
<!--stackedit_data:
eyJoaXN0b3J5IjpbMTMzNjI4NjkwNF19
-->