СЛОЖНЫЙ ПРИМЕР

$$2 * ( \frac{3}{4} - \frac{5}{6} ) * \frac{7}{8} = 2 * ( \frac{3 * 6}{4 * 6} - \frac{5 * 4}{6 * 4} ) * \frac{7}{8} = 2 * ( \frac{18}{24} - \frac{20}{24} ) * \frac{7}{8} = 2 * ( \frac{18 - 20}{24} ) * \frac{7}{8} = 2 * ( \frac{- 2}{24} ) * \frac{7}{8} = = 2 * \frac{( - 1 ) * 2}{24} * \frac{7}{8} = ( - 1 ) * 2 * \frac{2}{24} * \frac{7}{8} = ( - 1 ) * 2 * \frac{1}{12} * \frac{7}{8} = ( - 1 ) * 2 * \frac{1 * 7}{12 * 8} = = ( - 1 ) * 2 * \frac{7}{96} = ( - 1 ) * \frac{7 * 2}{48 * 2} = ( - 1 ) * \frac{7}{48} = - \frac{7}{48}$$

Можно было поступить быстрее

$$2 * ( \frac{3 * 6}{4 * 6} - \frac{5 * 4}{6 * 4} ) * \frac{7}{8} = ( \frac{18 - 20}{24} ) * \frac{2 * 7}{8} = \frac{- 2}{24} * \frac{7}{4} = - \frac{1 * 7}{12 * 4} = - \frac{7}{48}$$

$$8 * ( \frac{7}{6} - \frac{5}{4} ) * \frac{3}{2} = 8 * ( \frac{7 * 4}{6 * 4} - \frac{5 * 6}{4 * 6} ) * \frac{3}{2} = ( \frac{28}{24} - \frac{30}{24} ) * \frac{8 * 3}{2} = ( \frac{28 - 30}{24} ) * \frac{24}{2} = \frac{- 2}{24} * \frac{24}{2} = \frac{- 1 * 2 * 24}{24 * 2} = - 1$$

Все задания ниже можно вычислить быстро.

Осталось понять как…

$$3.17 + 10.2 + 0.83 + 9.8 =$$

$$15.21 - 3.9 - 4.7 + 6.79 =$$

$$50 * 1.34 * 0.2 =$$

$$- 75.7 * 0.5 * 20 =$$

$$25 * ( - 15.8) * 4 =$$

$$0.47 * 0.4 * 25 =$$

$$( 1.25 * 1.7 * 0.8 - 1.7 ) * 3.45 =$$

$$3.947:( 3.6 - 2.6 * 4 * 0.25 ) =$$

Еще задания
$$0.6\ *\ 2\ *\ ( - 3 + 5.2) - 4 =$$

$$\frac{2.7}{- 0.03} - \frac{12}{40} + 6 - ( - 3) =$$

$$\frac{128}{- 2} + 8\ *\ ( - 8 ) + \frac{6.8}{4} =$$

$$- 4 + \frac{20}{- 16} + \frac{4.2}{( - 0.7 )} + ( - 2) =$$

$$120 - 90\ *\ ( - 0.02 ) - \frac{15}{3} + \frac{96}{( - 4 )} =$$
